\section{Formulation des Ã©quations de Maxwell}

Dans le vide, on a \(\eps=\eps_0\), \(\mu=\mu_0\), \(\eta_0 = \sqrt{\mu_0 \slash \eps_0}\)

\begin{equation}
\left\lbrace \begin{matrix}
\vrot \vE + i\w\mu \vH &=& 0 \\
\vrot \vH - i\w\eps \vE &=& 0 \\
\end{matrix} \right.
\end{equation}

On pose \(\mu_r = \mu \slash \mu_0\), \(\eps_r = \eps \slash \eps_0\), \(k_0 = \w \sqrt {\eps_0\mu_0}\),

\begin{equation}
\left\lbrace \begin{matrix}
\vrot \vE + ik_0\eta_0\mu_r \vH &=& 0 \\
\vrot \vH - ik_0\eta_0^{-1}\eps_r \vE &=& 0 \\
\end{matrix} \right.
\quad
\overset{\vH' = \eta_0 \vH}{\Rightarrow}
\quad
\left\lbrace \begin{matrix}
\vrot \vE + ik_0\mu_r \vH' &=& 0 \\
\vrot \vH' - ik_0\eps_r \vE &=& 0 \\
\end{matrix} \right.
\end{equation}

On pose \(k=k_0\nu_r\), \(\nu_r = \sqrt{\mu_r\eps_r}\), \(\eta_r = \sqrt{\mu_r \slash \eps_r}\)

\begin{equation}
\left\lbrace \begin{matrix}
\vrot \vE + ik\eta_0\eta_r \vH &=& 0 \\
\vrot \vH - ik\eta_0^{-1}\eta_r^{-1} \vE &=& 0 \\
\end{matrix} \right.
\quad
\overset{\vH' = \eta_0 \vH}{\Rightarrow}
\quad
\left\lbrace \begin{matrix}
\vrot \vE + ik\eta_r \vH' &=& 0 \\
\vrot \vH' - ik\eta_r^{-1} \vE &=& 0 \\
\end{matrix} \right.
\end{equation}